atomics/SC_atomics.v
@@ -17,29 +17,17 @@ Section SC_atomics.
 
 Context {CS : compspecs}.
 
-Definition AL_type := ProdType (ProdType (ProdType (ProdType (ProdType (ProdType (ConstType val) Mpred)
-  (ArrowType (ConstType iname) (ConstType Prop))) (ArrowType (ConstType iname) (ConstType Prop)))
-  (ArrowType (ConstType share) (ArrowType (ConstType Z) Mpred))) (ArrowType (ConstType Z) Mpred))
-  (ConstType invG).
-
-(*    SEP (|={Eo,Ei}=> EX sh : share, EX v : Z, !!(readable_share sh /\ repable_signed v) &&
-              data_at sh tint (vint v) p * (data_at sh tint (vint v) p -* |={Ei,Eo}=> Q v)) *)
-
-(*    SEP (|={Eo,Ei}=> EX sh : share, EX v : Z, !!(readable_share sh /\ repable_signed v) &&
-              data_at sh tint (vint v) p * (data_at sh tint (vint v') p -* |={Ei,Eo}=> Q)) *)
-
+Definition AL_type := ProdType (ProdType (ProdType (ProdType (ConstType val)
+  (ConstType coPset)) (ConstType coPset))
+  (ArrowType (ConstType Z) Mpred)) (ConstType invG).
 
 Program Definition load_SC_spec := TYPE AL_type
-  WITH p : val, P : mpred, Eo : Ensemble iname, Ei : Ensemble iname,
-       P' : share -> Z -> mpred, Q : Z -> mpred, inv_names : invG
+  WITH p : val, Eo : coPset, Ei : coPset, Q : Z -> mpred, inv_names : invG
   PRE [ 1%positive OF tptr tint ]
-   PROP (Included Ei Eo)
+   PROP (subseteq Ei Eo)
    LOCAL (temp 1%positive p)
-   SEP (P -* |={Eo,Ei}=> EX sh : share, EX v : Z, !!(readable_share sh /\ repable_signed v) &&
-              data_at sh tint (vint v) p * P' sh v;
-         ALL sh : _, ALL v : _, (!!(readable_share sh /\ repable_signed v) &&
-           data_at sh tint (vint v) p * P' sh v) -* |={Ei,Eo}=> Q v;
-         P)
+   SEP (|={Eo,Ei}=> EX sh : share, EX v : Z, !!(readable_share sh /\ repable_signed v) &&
+              data_at sh tint (vint v) p * (data_at sh tint (vint v) p -* |={Ei,Eo}=> Q v))%I
   POST [ tint ]
    EX v : Z,
    PROP (repable_signed v)
@@ -48,42 +36,34 @@ Program Definition load_SC_spec := TYPE AL_type
 Next Obligation.
 Proof.
   repeat intro.
-  destruct x as ((((((?, ?), ?), ?), ?), ?), ?); simpl.
+  destruct x as ((((?, ?), ?), ?), ?); simpl.
   unfold PROPx, LOCALx, SEPx; simpl; rewrite !approx_andp; f_equal;
-    f_equal; rewrite !sepcon_emp, ?approx_sepcon, ?approx_idem.
-  f_equal.
-  - setoid_rewrite fview_shift_nonexpansive; rewrite approx_idem; do 3 apply f_equal.
-    rewrite !approx_exp; apply f_equal; extensionality sh.
-    rewrite !approx_exp; apply f_equal; extensionality v.
-    rewrite !approx_sepcon, approx_idem; auto.
-  - f_equal.
-    rewrite !(approx_allp _ _ _ Share.bot); apply f_equal; extensionality sh.
-    rewrite !(approx_allp _ _ _ 0); apply f_equal; extensionality v.
-    setoid_rewrite fview_shift_nonexpansive; rewrite approx_idem; apply f_equal; f_equal.
-    rewrite !approx_sepcon, approx_idem; auto.
+    f_equal; rewrite -> !sepcon_emp, ?approx_sepcon, ?approx_idem.
+  setoid_rewrite fupd_nonexpansive; do 2 f_equal.
+  rewrite !approx_exp; apply f_equal; extensionality sh.
+  rewrite !approx_exp; apply f_equal; extensionality v. 
+  rewrite !approx_sepcon; f_equal.
+  setoid_rewrite fview_shift_nonexpansive; rewrite approx_idem; auto.
 Qed.
 Next Obligation.
 Proof.
   repeat intro.
-  destruct x as ((((((?, ?), ?), ?), ?), ?), ?); simpl.
+  destruct x as ((((?, ?), ?), ?), ?); simpl.
   rewrite !approx_exp; apply f_equal; extensionality v.
   unfold PROPx, LOCALx, SEPx; simpl; rewrite !approx_andp; do 2 apply f_equal;
-    rewrite !sepcon_emp, ?approx_sepcon, ?approx_idem; auto.
+    rewrite -> !sepcon_emp, ?approx_sepcon, ?approx_idem; auto.
 Qed.
 
-Definition AS_type := ProdType (ProdType (ProdType (ProdType (ProdType (ProdType (ConstType (val * Z)) Mpred)
-  (ArrowType (ConstType iname) (ConstType Prop))) (ArrowType (ConstType iname) (ConstType Prop)))
-  (ArrowType (ConstType share) Mpred)) Mpred)
-  (ConstType invG).
+Definition AS_type := ProdType (ProdType (ProdType (ProdType (ConstType (val * Z))
+  (ConstType coPset)) (ConstType coPset)) Mpred) (ConstType invG).
 
 Program Definition store_SC_spec := TYPE AS_type
-  WITH p : val, v : Z, P : mpred, Eo : Ensemble iname, Ei : Ensemble iname,
-       P' : share -> mpred, Q : mpred, inv_names : invG
+  WITH p : val, v : Z, Eo : coPset, Ei : coPset, Q : mpred, inv_names : invG
   PRE [ 1%positive OF tptr tint, 2%positive OF tint ]
-   PROP (repable_signed v)
+   PROP (repable_signed v; subseteq Ei Eo)
    LOCAL (temp 1%positive p; temp 2%positive (vint v))
-   SEP (P -* |={Eo,Ei}=> EX sh : share, !!(writable_share sh) && data_at_ sh tint p * P' sh;
-        ALL sh : _, (!!(writable_share sh) && data_at sh tint (vint v) p * P' sh) -* |={Ei,Eo}=> Q; P)
+   SEP (|={Eo,Ei}=> EX sh : share, !!(writable_share sh) && data_at_ sh tint p *
+      (data_at sh tint (vint v) p -* |={Ei,Eo}=> Q))%I
   POST [ tvoid ]
    PROP ()
    LOCAL ()
@@ -91,45 +71,34 @@ Program Definition store_SC_spec := TYPE AS_type
 Next Obligation.
 Proof.
   repeat intro.
-  destruct x as (((((((?, ?), ?), ?), ?), ?), ?), ?); simpl.
+  destruct x as (((((?, ?), ?), ?), ?), ?); simpl.
   unfold PROPx, LOCALx, SEPx; simpl; rewrite !approx_andp; f_equal;
-    f_equal; rewrite !sepcon_emp, ?approx_sepcon, ?approx_idem.
-  f_equal.
-  - setoid_rewrite fview_shift_nonexpansive; rewrite approx_idem; do 3 apply f_equal.
-    rewrite !approx_exp; apply f_equal; extensionality sh.
-    rewrite !approx_sepcon, approx_idem; auto.
-  - f_equal.
-    rewrite !(approx_allp _ _ _ Share.bot); apply f_equal; extensionality sh.
-    setoid_rewrite fview_shift_nonexpansive; rewrite approx_idem; apply f_equal; f_equal.
-    rewrite !approx_sepcon, approx_idem; auto.
+    f_equal; rewrite -> !sepcon_emp, ?approx_sepcon, ?approx_idem.
+  setoid_rewrite fupd_nonexpansive; do 2 f_equal.
+  rewrite !approx_exp; apply f_equal; extensionality sh.
+  rewrite !approx_sepcon; f_equal.
+  setoid_rewrite fview_shift_nonexpansive; rewrite approx_idem; auto.
 Qed.
 Next Obligation.
 Proof.
   repeat intro.
-  destruct x as (((((((?, ?), ?), ?), ?), ?), ?), ?); simpl.
+  destruct x as (((((?, ?), ?), ?), ?), ?); simpl.
   unfold PROPx, LOCALx, SEPx; simpl; rewrite !approx_andp; do 2 apply f_equal;
-    rewrite !sepcon_emp, ?approx_sepcon, ?approx_idem; auto.
+    rewrite -> !sepcon_emp, ?approx_sepcon, ?approx_idem; auto.
 Qed.
 
-Definition ACAS_type := ProdType (ProdType (ProdType (ProdType (ProdType (ProdType (ConstType (val * Z * Z)) Mpred)
-  (ArrowType (ConstType iname) (ConstType Prop))) (ArrowType (ConstType iname) (ConstType Prop)))
-  (ArrowType (ConstType share) (ArrowType (ConstType Z) Mpred))) (ArrowType (ConstType Z) Mpred))
-  (ConstType invG).
-
-(* |={Eo,Ei}=> EX sh : share, EX v0 : Z, !!(writable_share sh /\ repable_signed v0) &&
-              data_at sh tint (vint v0) p *
-      (data_at sh tint (vint (if eq_dec v0 c then v else v0)) p -* |={Ei,Eo}=> Q v0) *)
+Definition ACAS_type := ProdType (ProdType (ProdType (ProdType (ConstType (val * Z * Z))
+  (ConstType coPset)) (ConstType coPset))
+  (ArrowType (ConstType Z) Mpred)) (ConstType invG).
 
 Program Definition CAS_SC_spec := TYPE ACAS_type
-  WITH p : val, c : Z, v : Z, P : mpred, Eo : Ensemble iname, Ei : Ensemble iname,
-       P' : share -> Z -> mpred, Q : Z -> mpred, inv_names : invG
+  WITH p : val, c : Z, v : Z, Eo : coPset, Ei : coPset, Q : Z -> mpred, inv_names : invG
   PRE [ 1%positive OF tptr tint, 2%positive OF tint, 3%positive OF tint ]
-   PROP (repable_signed c; repable_signed v)
+   PROP (repable_signed c; repable_signed v; subseteq Ei Eo)
    LOCAL (temp 1%positive p; temp 2%positive (vint c); temp 3%positive (vint v))
-   SEP (P -* |={Eo,Ei}=> EX sh : share, EX v0 : Z, !!(writable_share sh /\ repable_signed v0) &&
-              data_at sh tint (vint v0) p * P' sh v0;
-         ALL sh : _, ALL v0 : _, (!!(writable_share sh /\ repable_signed v0) &&
-           data_at sh tint (vint (if eq_dec v0 c then v else v0)) p * P' sh v0) -* |={Ei,Eo}=> Q v0; P)
+   SEP (|={Eo,Ei}=> EX sh : share, EX v0 : Z, !!(writable_share sh /\ repable_signed v0) &&
+              data_at sh tint (vint v0) p *
+           (data_at sh tint (vint (if eq_dec v0 c then v else v0)) p -* |={Ei,Eo}=> Q v0))%I
   POST [ tint ]
    EX v' : Z,
    PROP (repable_signed v')
@@ -138,44 +107,36 @@ Program Definition CAS_SC_spec := TYPE ACAS_type
 Next Obligation.
 Proof.
   repeat intro.
-  destruct x as ((((((((?, ?), ?), ?), ?), ?), ?), ?), ?); simpl.
+  destruct x as ((((((?, ?), ?), ?), ?), ?), ?); simpl.
   unfold PROPx, LOCALx, SEPx; simpl; rewrite !approx_andp; f_equal;
-    f_equal; rewrite !sepcon_emp, ?approx_sepcon, ?approx_idem.
-  f_equal.
-  - setoid_rewrite fview_shift_nonexpansive; rewrite approx_idem; do 3 apply f_equal.
-    rewrite !approx_exp; apply f_equal; extensionality sh.
-    rewrite !approx_exp; apply f_equal; extensionality v0.
-    rewrite !approx_sepcon, approx_idem; auto.
-  - f_equal.
-    rewrite !(approx_allp _ _ _ Share.bot); apply f_equal; extensionality sh.
-    rewrite !(approx_allp _ _ _ 0); apply f_equal; extensionality v0.
-    setoid_rewrite fview_shift_nonexpansive; rewrite approx_idem; apply f_equal; f_equal.
-    rewrite !approx_sepcon, approx_idem; auto.
+    f_equal; rewrite -> !sepcon_emp, ?approx_sepcon, ?approx_idem.
+  setoid_rewrite fupd_nonexpansive; do 2 f_equal.
+  rewrite !approx_exp; apply f_equal; extensionality sh.
+  rewrite !approx_exp; apply f_equal; extensionality v0.
+  rewrite !approx_sepcon; f_equal.
+  setoid_rewrite fview_shift_nonexpansive; rewrite approx_idem; auto.
 Qed.
 Next Obligation.
 Proof.
   repeat intro.
-  destruct x as ((((((((?, ?), ?), ?), ?), ?), ?), ?), ?); simpl.
+  destruct x as ((((((?, ?), ?), ?), ?), ?), ?); simpl.
   rewrite !approx_exp; apply f_equal; extensionality vr.
   unfold PROPx, LOCALx, SEPx; simpl; rewrite !approx_andp; do 2 apply f_equal;
-    rewrite !sepcon_emp, ?approx_sepcon, ?approx_idem; auto.
+    rewrite -> !sepcon_emp, ?approx_sepcon, ?approx_idem; auto.
 Qed.
 
-Definition AEX_type := ProdType (ProdType (ProdType (ProdType (ProdType (ProdType (ConstType (val * Z)) Mpred)
-  (ArrowType (ConstType iname) (ConstType Prop))) (ArrowType (ConstType iname) (ConstType Prop)))
-  (ArrowType (ConstType share) (ArrowType (ConstType Z) Mpred))) (ArrowType (ConstType Z) Mpred))
-  (ConstType invG).
+Definition AEX_type := ProdType (ProdType (ProdType (ProdType (ConstType (val * Z))
+  (ConstType coPset)) (ConstType coPset))
+  (ArrowType (ConstType Z) Mpred)) (ConstType invG).
 
 Program Definition AEX_SC_spec := TYPE AEX_type
-  WITH p : val, v : Z, P : mpred, Eo : Ensemble iname, Ei : Ensemble iname,
-       P' : share -> Z -> mpred, Q : Z -> mpred, inv_names : invG
+  WITH p : val, v : Z, Eo : coPset, Ei : coPset, Q : Z -> mpred, inv_names : invG
   PRE [ 1%positive OF tptr tint, 2%positive OF tint ]
-   PROP (repable_signed v)
+   PROP (repable_signed v; subseteq Ei Eo)
    LOCAL (temp 1%positive p; temp 2%positive (vint v))
-   SEP (P -* |={Eo,Ei}=> EX sh : share, EX v0 : Z, !!(writable_share sh /\ repable_signed v0) &&
-              data_at sh tint (vint v0) p * P' sh v0;
-        ALL sh : _, ALL v0 : _, (!!(writable_share sh /\ repable_signed v0) &&
-           data_at sh tint (vint v) p * P' sh v0) -* |={Ei,Eo}=> Q v0; P)
+   SEP (|={Eo,Ei}=> EX sh : share, EX v0 : Z, !!(writable_share sh /\ repable_signed v0) &&
+              data_at sh tint (vint v0) p *
+        (data_at sh tint (vint v) p -* |={Ei,Eo}=> Q v0))%I
   POST [ tint ]
    EX v' : Z,
    PROP (repable_signed v')
@@ -184,40 +145,22 @@ Program Definition AEX_SC_spec := TYPE AEX_type
 Next Obligation.
 Proof.
   repeat intro.
-  destruct x as (((((((?, ?), ?), ?), ?), ?), ?), ?); simpl.
+  destruct x as (((((?, ?), ?), ?), ?), ?); simpl.
   unfold PROPx, LOCALx, SEPx; simpl; rewrite !approx_andp; f_equal;
-    f_equal; rewrite !sepcon_emp, ?approx_sepcon, ?approx_idem.
-  f_equal.
-  - setoid_rewrite fview_shift_nonexpansive; rewrite approx_idem; do 3 apply f_equal.
-    rewrite !approx_exp; apply f_equal; extensionality sh.
-    rewrite !approx_exp; apply f_equal; extensionality v0.
-    rewrite !approx_sepcon, approx_idem; auto.
-  - f_equal.
-    rewrite !(approx_allp _ _ _ Share.bot); apply f_equal; extensionality sh.
-    rewrite !(approx_allp _ _ _ 0); apply f_equal; extensionality v0.
-    setoid_rewrite fview_shift_nonexpansive; rewrite approx_idem; apply f_equal; f_equal.
-    rewrite !approx_sepcon, approx_idem; auto.
+    f_equal; rewrite -> !sepcon_emp, ?approx_sepcon, ?approx_idem.
+  setoid_rewrite fupd_nonexpansive; do 2 f_equal.
+  rewrite !approx_exp; apply f_equal; extensionality sh.
+  rewrite !approx_exp; apply f_equal; extensionality v0.
+  rewrite !approx_sepcon; f_equal.
+  setoid_rewrite fview_shift_nonexpansive; rewrite approx_idem; auto.
 Qed.
 Next Obligation.
 Proof.
   repeat intro.
-  destruct x as (((((((?, ?), ?), ?), ?), ?), ?), ?); simpl.
+  destruct x as (((((?, ?), ?), ?), ?), ?); simpl.
   rewrite !approx_exp; apply f_equal; extensionality vr.
   unfold PROPx, LOCALx, SEPx; simpl; rewrite !approx_andp; do 2 apply f_equal;
-    rewrite !sepcon_emp, ?approx_sepcon, ?approx_idem; auto.
+    rewrite -> !sepcon_emp, ?approx_sepcon, ?approx_idem; auto.
 Qed.
 
 End SC_atomics.
-
-Notation store_SC_witness p v P Eo Ei Q invG := (p, v%Z, P, Eo, Ei,
-  fun sh => !!(writable_share sh) && data_at sh tint (vint v) p -* Q, Q, invG).
-
-Notation AEX_SC_witness p v P Eo Ei Q invG := (p, v%Z, P, Eo, Ei,
-  fun sh v0 => !!(writable_share sh /\ repable_signed v0) && data_at sh tint (vint v) p -* Q v0, Q, invG).
-
-Notation load_SC_witness p P Eo Ei Q invG := (p, P, Eo, Ei,
-  fun sh v => !!(readable_share sh /\ repable_signed v) && data_at sh tint (vint v) p -* Q v, Q, invG).
-
-Notation CAS_SC_witness p c v P Eo Ei Q invG := (p, c, v%Z, P, Eo, Ei,
-  fun sh v0 => !!(writable_share sh /\ repable_signed v0) &&
-    data_at sh tint (vint (if eq_dec v0 c then v else v0)) p -* Q v0, Q, invG).
